Quicksort: refactor Par version, add basic TaskParallel version

pulse/share/steel/examples/pulse/QuicksortParallel.fst
@@ -22,31 +22,57 @@ module T = FStar.Tactics
 module SZ = FStar.SizeT
 
 let nat_smaller (n: nat) = i:nat{i < n}
-let seqn (n: nat) = (s:Seq.seq int{Seq.length s = n})
-let arrayn (n: nat) = (a:A.array int{A.length a = n})
 let nat_fits = n:nat{SZ.fits n}
 
 let seq_swap (#a: Type) (s: Seq.seq a) (i j: nat_smaller (Seq.length s)) =
   Seq.swap s j i
 
 let larger_than (s: Seq.seq int) (lb: int)
-  = forall (k: nat). k < Seq.length s ==> lb <= Seq.index s k
-
-let larger_than_slice (s: Seq.seq int) (lo: nat) (hi: nat{lo <= hi /\ hi <= Seq.length s}) (lb: int):
-  Lemma (requires larger_than s lb)
-  (ensures larger_than (Seq.slice s lo hi) lb)
-= ()
+  = forall (k: int). 0 <= k /\ k < Seq.length s ==> lb <= Seq.index s k
 
 let smaller_than (s: Seq.seq int) (rb: int)
-  = forall (k: nat). k < Seq.length s ==> Seq.index s k <= rb
+  = forall (k: int). 0 <= k /\ k < Seq.length s ==> Seq.index s k <= rb
 
 let between_bounds (s: Seq.seq int) (lb rb: int)
   = larger_than s lb /\ smaller_than s rb
 
+let sorted (s: Seq.seq int)
+  = forall (i j: nat). i <= j /\ j < Seq.length s ==> Seq.index s i <= Seq.index s j
+
+let lemma_sorted_append
+  (s1 s2 : Seq.seq int)
+  (l1 r1 l2 r2 : int)
+  : Lemma
+    (requires sorted s1 /\ between_bounds s1 l1 r1 /\
+              sorted s2 /\ between_bounds s2 l2 r2 /\
+              r1 >= l1 /\ r2 >= l2 /\ // silly, but needed since the seqs may be empty
+              r1 <= l2)
+    (ensures sorted (Seq.append s1 s2) /\ between_bounds (Seq.append s1 s2) l1 r2)
+  = ()
+
+let lemma_sorted_append_squash
+  (s1 s2 : Seq.seq int)
+  (l1 r1 l2 r2 : int)
+    (_ : squash (sorted s1 /\ between_bounds s1 l1 r1 /\
+              sorted s2 /\ between_bounds s2 l2 r2 /\
+              r1 >= l1 /\ r2 >= l2 /\ // silly, but needed since the seqs may be empty
+              r1 <= l2))
+    : squash (sorted (Seq.append s1 s2) /\ between_bounds (Seq.append s1 s2) l1 r2)
+  = ()
+
+let to_nat (x: int{x >= 0}): nat = x
 (** Permutation reasoning **)
 
 [@@"opaque_to_smt"]
-let permutation = Seq.Properties.permutation int
+let permutation s1 s2 : prop = (Seq.Properties.permutation int s1 s2)
+
+let permutation_same_length (s1 s2 : Seq.seq int)
+  : Lemma (requires permutation s1 s2)
+          (ensures Seq.length s1 == Seq.length s2)
+          [SMTPat (permutation s1 s2)]
+  = 
+  reveal_opaque (`%permutation) (permutation s1 s2);
+  Seq.Properties.perm_len s1 s2
 
 let append_permutations_3 (s1 s2 s3 s1' s3': Seq.seq int):
   Lemma
@@ -60,6 +86,12 @@ let append_permutations_3 (s1 s2 s3 s1' s3': Seq.seq int):
   reveal_opaque (`%permutation) (permutation (Seq.append s1 (Seq.append s2 s3)) (Seq.append s1' (Seq.append s2 s3')));
   Seq.Properties.append_permutations s1 (Seq.append s2 s3) s1' (Seq.append s2 s3')
   )
+
+(* workaround for #151 *)
+let append_permutations_3_squash (s1 s2 s3 s1' s3': Seq.seq int)
+  (_ : squash (permutation s1 s1' /\ permutation s3 s3'))
+  : squash (permutation (Seq.append s1 (Seq.append s2 s3)) (Seq.append s1' (Seq.append s2 s3')))
+= append_permutations_3 s1 s2 s3 s1' s3'
 
 let seq_swap_commute (s: Seq.seq int) (i j: nat_smaller (Seq.length s)):
   Lemma (seq_swap s i j == seq_swap s j i)
@@ -132,7 +164,6 @@ let op_Array_Assignment
   (v: t)
   (#l: nat{l <= SZ.v i})
   (#r: nat{SZ.v i < r})
-  //(#s: Ghost.erased (Seq.seq t) {US.v i < Seq.length s})
   (#s0: Ghost.erased (Seq.seq t))
 : stt unit
     (requires A.pts_to_range a l r s0)
@@ -150,10 +181,12 @@ let op_Array_Assignment
 fn swap (a: A.array int) (i j: nat_fits) (#l:(l:nat{l <= i /\ l <= j})) (#r:(r:nat{i < r /\ j < r}))
   (#s0: Ghost.erased (Seq.seq int))
   requires A.pts_to_range a l r s0
-  ensures exists* s. (A.pts_to_range a l r s
-    ** pure (Seq.length s0 = r - l /\ Seq.length s = r - l /\
-      s = seq_swap s0 (i - l) (j - l) /\ permutation s0 s
-    ))
+  ensures
+    exists* s. 
+      A.pts_to_range a l r s **
+      pure (Seq.length s0 = r - l /\
+            s == seq_swap s0 (i - l) (j - l) /\
+            permutation s0 s)
 {
   let vi = a.(SZ.uint_to_t i);
   let vj = a.(SZ.uint_to_t j);
@@ -163,46 +196,36 @@ fn swap (a: A.array int) (i j: nat_fits) (#l:(l:nat{l <= i /\ l <= j})) (#r:(r:n
 }
 ```
 
-let sorted (s: Seq.seq int)
-  = forall (i j: nat). 0 <= i /\ i <= j /\ j < Seq.length s ==> Seq.index s i <= Seq.index s j
-
-let to_nat (x: int{x >= 0}): nat = x
-
-#push-options "--z3rlimit 50"
-
-(* Proof below is flaky for whatever reason on 4.8.5, but not
-4.12.3. Use this for now. *)
-#restart-solver
-
 ```pulse
-fn partition (a: A.array int) (lo: nat) (hi:(hi:nat{lo < hi - 1})) (n: nat) (lb rb: int) (#s0: Ghost.erased (Seq.seq int))
+fn partition (a: A.array int) (lo: nat) (hi:(hi:nat{lo < hi}))
+  (lb rb: erased int)
+  (#s0: Ghost.erased (Seq.seq int))
   requires (
     A.pts_to_range a lo hi s0 **
     pure (
-      hi - 1 < n /\
-      n = A.length a /\ SZ.fits n /\
+      hi <= A.length a /\
+      SZ.fits (A.length a) /\
       Seq.length s0 = hi - lo /\
       between_bounds s0 lb rb
       )
   )
-  returns r: nat & nat & int // left, right, pivot
-  ensures exists* s. (
-    A.pts_to_range a lo hi s
-     **
+  returns r: nat & nat & int // left index, right index, pivot value
+  ensures exists* s.
+    A.pts_to_range a lo hi s **
     pure (
       Seq.length s = hi - lo /\ Seq.length s0 = hi - lo
-      /\ lo <= r._1 /\ r._1 < r._2 /\ r._2 <= hi /\ hi - 1 < n
+      /\ lo <= r._1 /\ r._1 < r._2 /\ r._2 <= hi /\ hi <= A.length a
       /\ lb <= r._3 /\ r._3 <= rb
-      /\ (forall (k: nat). k < r._1 - lo ==> Seq.index s k < r._3)
-      /\ (forall (k: nat). r._1 - lo <= k /\ k <= r._2 - 1 - lo ==> Seq.index s k == r._3)
-      /\ (forall (k: nat). r._2 - lo <= k /\ k <= hi - 1 - lo ==> Seq.index s k > r._3)
+      /\ (forall (k: nat).   lo <= k /\ k < r._1  ==> Seq.index s (k - lo) <  r._3)
+      /\ (forall (k: nat). r._1 <= k /\ k < r._2  ==> Seq.index s (k - lo) == r._3)
+      /\ (forall (k: nat). r._2 <= k /\ k < hi    ==> Seq.index s (k - lo) >  r._3)
       /\ between_bounds s lb rb
       /\ permutation s0 s
-   ))
+    )
 {
   let pivot = a.(SZ.uint_to_t (hi - 1));
-  let mut i = lo - 1;
-  let mut j = lo - 1;
+  let mut i = lo;
+  let mut j = lo;
   let mut k = lo;
   while (let vk = !k; (vk < hi - 1))
     invariant b . exists* s vi vj vk. (
@@ -214,13 +237,13 @@ fn partition (a: A.array int) (lo: nat) (hi:(hi:nat{lo < hi - 1})) (n: nat) (lb 
         b == (vk < hi - 1) /\
         //eq2_prop #bool b (vk < hi - 1) /\
         lo <= vk /\ vk <= hi - 1 /\
-        lo - 1 <= vi /\ vi <= vj /\ vj < vk /\
+        lo <= vi /\ vi <= vj /\ vj <= vk /\
         lb <= pivot /\ pivot <= rb /\
         Seq.length s = hi - lo /\
         Seq.index s (hi - 1 - lo) = pivot
-        /\ (forall (l:nat). 0 <= l /\ l <= vi - lo ==> Seq.index s l < pivot)
-        /\ (forall (l:nat). vi + 1 - lo <= l /\ l <= vj - lo ==> Seq.index s l == pivot)
-        /\ (forall (l:nat). vj + 1 - lo <= l /\ l <= vk - 1 - lo ==> Seq.index s l > pivot)
+        /\ (forall (l: nat). lo <= l /\ l < vi ==> Seq.index s (l - lo) <  pivot)
+        /\ (forall (l: nat). vi <= l /\ l < vj ==> Seq.index s (l - lo) == pivot)
+        /\ (forall (l: nat). vj <= l /\ l < vk ==> Seq.index s (l - lo) >  pivot)
         /\ permutation s0 s
         /\ between_bounds s lb rb
       ))
@@ -229,107 +252,139 @@ fn partition (a: A.array int) (lo: nat) (hi:(hi:nat{lo < hi - 1})) (n: nat) (lb 
     let ak = a.(SZ.uint_to_t vk);
     if (ak < pivot) {
       let vi = !i;
-      i := vi + 1;
       let vj = !j;
+      swap a vj vk;
+      swap a vi vj;
+      i := vi + 1;
       j := vj + 1;
-      swap a (vj + 1) vk;
-      swap a (vi + 1) (vj + 1);
       k := vk + 1;
-      ()
-    }
-    else {
-      if (ak = pivot) {
-        let vj = !j;
-        j := vj + 1;
-        swap a (vj + 1) vk;
-        k := vk + 1;
-        ()
-      }
-      else {
-        k := vk + 1;
-        ()
-      };
+    } else if (ak = pivot) {
+      let vj = !j;
+      swap a vj vk;
+      j := vj + 1;
+      k := vk + 1;
+    } else {
+      k := vk + 1;
     };
   };
 
-  let vj = !j;
-  j := vj + 1;
+  let vi  : nat = !i;
+  let vj  : nat = !j;
+  let vj' : nat = vj + 1;
 
-  // swap j with hi
-  swap a (vj + 1) (hi - 1);
-
-  let vi = !i;
-  i := vi + 1;
-  let vi' = to_nat (vi + 1);
-  let vj' = to_nat (vj + 2);
-  (vi', vj', pivot)
+  // swap j with hi, essentially transition from shape
+  //  [ < < < < = = = = > > > > p ]
+  // to shape:
+  //  [ < < < < = = = = p > > > > ]
+  // where < = > represent values that are less than, equal, and greater than the pivot p
+  swap a vj (hi - 1);
+  (vi, vj', pivot)
 }
 ```
+
+#push-options "--retry 5"
+let transfer_larger_slice
+  (s : Seq.seq int)
+  (shift : nat)
+  (l : nat{shift <= l})
+  (r : nat{l <= r /\ r <= shift + Seq.length s})
+  (lb: int)
+: Lemma
+    (requires 
+      forall (k: int). l <= k /\ k < r ==> (lb <= Seq.index s (k - shift))
+    )
+    (ensures larger_than (Seq.slice s (l - shift) (r - shift)) lb)
+= assert (forall (k: int). l <= k /\ k < r ==> (lb <= Seq.index s (k - shift)));
+  assert (forall (k: int). l <= (k+shift) /\ (k+shift) < r ==> (lb <= Seq.index s ((k+shift) - shift)));
+  assert (forall (k: int). l - shift <= k /\ k < r - shift ==> (lb <= Seq.index s k));
+  ()
+
+let transfer_smaller_slice
+  (s : Seq.seq int)
+  (shift : nat)
+  (l : nat{shift <= l})
+  (r : nat{l <= r /\ r <= shift + Seq.length s})
+  (rb: int)
+: Lemma
+    (requires 
+      forall (k: int). l <= k /\ k < r ==> (Seq.index s (k - shift) <= rb)
+    )
+    (ensures smaller_than (Seq.slice s (l - shift) (r - shift)) rb)
+= assert (forall (k: int). l <= k /\ k < r ==> (Seq.index s (k - shift) <= rb));
+  assert (forall (k: int). l <= (k+shift) /\ (k+shift) < r ==> (Seq.index s ((k+shift) - shift) <= rb));
+  assert (forall (k: int). l - shift <= k /\ k < r - shift ==> (Seq.index s k <= rb));
+  ()
 #pop-options
 
-let transfer_larger_slice (s: Seq.seq int) (l: nat) (r: nat{l <= r /\ r <= Seq.length s}) (lb: int):
-  Lemma
-    (requires (forall (k: nat). l <= k /\ k < r ==> (lb <= Seq.index s k)))
-    (ensures larger_than (Seq.slice s l r) lb)
-= ()
-
-let transfer_smaller_slice (s: Seq.seq int) (l: nat) (r: nat{l <= r /\ r <= Seq.length s}) (rb: int):
-  Lemma
-    (requires (forall (k: nat). l <= k /\ k < r ==> (Seq.index s k <= rb)))
-    (ensures smaller_than (Seq.slice s l r) rb)
-= ()
+let transfer_equal_slice
+  (s : Seq.seq int)
+  (shift : nat)
+  (l : nat{shift <= l})
+  (r : nat{l <= r /\ r <= shift + Seq.length s})
+  (rb: int)
+: Lemma
+    (requires 
+      forall (k: int). l <= k /\ k < r ==> (Seq.index s (k - shift) == rb)
+    )
+    (ensures larger_than (Seq.slice s (l-shift) (r-shift)) rb /\
+             smaller_than (Seq.slice s (l - shift) (r - shift)) rb)
+= transfer_smaller_slice s shift l r rb;
+  transfer_larger_slice s shift l r rb;
+  ()
 
 #push-options "--z3rlimit 50"
 ```pulse
-fn partition_wrapper (a: A.array int) (lo: nat) (hi:(hi:nat{lo < hi - 1})) (n: nat) (lb rb: int) (#s0: Ghost.erased (Seq.seq int))
+fn partition_wrapper (a: A.array int) (lo: nat) (hi:(hi:nat{lo < hi}))
+  (lb rb: erased int)
+  (#s0: Ghost.erased (Seq.seq int))
   requires (
     A.pts_to_range a lo hi s0 **
-    pure (hi - 1 < n /\ n = A.length a /\ SZ.fits n /\ between_bounds s0 lb rb
-      /\ Seq.length s0 = hi - lo)
-  )
-  returns r: nat & nat & int // left, right, pivot
-  ensures exists* s1 s2 s3. (
-    A.pts_to_range a lo r._1 s1 **
-    A.pts_to_range a r._1 r._2 s2 **
-    A.pts_to_range a r._2 hi s3 **
     pure (
-      lo <= r._1 /\ r._1 < r._2 /\ r._2 <= hi /\ hi - 1 < n /\
+      hi <= A.length a /\
+      SZ.fits (A.length a) /\
+      Seq.length s0 = hi - lo /\
+      between_bounds s0 lb rb
+      )
+  )
+  returns r: nat & nat & int // left index, right index, pivot value
+  ensures exists* s1 s2 s3. (
+    A.pts_to_range a lo   r._1 s1 **
+    A.pts_to_range a r._1 r._2 s2 **
+    A.pts_to_range a r._2 hi   s3 **
+    pure (
+      lo <= r._1 /\ r._1 < r._2 /\ r._2 <= hi /\ hi <= A.length a /\
       lb <= r._3 /\ r._3 <= rb /\
-      Seq.length s1 = r._1 - lo /\ Seq.length s2 = r._2 - r._1 /\ Seq.length s3 = hi - r._2
+      Seq.length s1 == r._1 - lo /\ Seq.length s2 == r._2 - r._1 /\ Seq.length s3 == hi - r._2
       /\ between_bounds s1 lb r._3
       /\ between_bounds s2 r._3 r._3
       /\ between_bounds s3 r._3 rb
       /\ permutation s0 (Seq.append s1 (Seq.append s2 s3))
    ))
 {
-  let r = partition a lo hi n lb rb #s0;
+  let r = partition a lo hi lb rb #s0;
   with s. assert (A.pts_to_range a lo hi s);
 
-  transfer_smaller_slice s 0 (r._1 - lo) r._3;
-  transfer_larger_slice s (r._2 - lo) (hi - lo) r._3;
-
-  let pivot = r._3;
   pts_to_range_split a lo r._1 hi;
-  with s1. assert (A.pts_to_range a lo r._1 s1);
-  assert_prop (s1 == Seq.slice s 0 (r._1 - lo));
-
-  assert_prop (between_bounds s1 lb r._3);
-
-  with s23. assert (A.pts_to_range a r._1 hi s23);
-  assert_prop (s23 == Seq.slice s (r._1 - lo) (Seq.length s));
-
-  assert (A.pts_to_range a lo r._1 s1);
   pts_to_range_split a r._1 r._2 hi;
-
+  with s1. assert (A.pts_to_range a lo r._1 s1);
   with s2. assert (A.pts_to_range a r._1 r._2 s2);
-  assert_prop (s2 == Seq.slice s23 0 (r._2 - r._1));
-  assert_prop (s2 == Seq.slice s (r._1 - lo) (r._2 - lo));
   with s3. assert (A.pts_to_range a r._2 hi s3);
-  assert_prop (s3 == Seq.slice s (r._2 - lo) (hi - lo));
-  assert_prop (Seq.length s1 = r._1 - lo);
-  assert_prop (Seq.length s2 = r._2 - r._1);
-  assert_prop (Seq.length s3 = hi - r._2);
-  assert_prop (s == Seq.append s1 (Seq.append s2 s3));
+  
+  assert (pure (Seq.length s1 == r._1 - lo));
+  assert (pure (Seq.length s2 == r._2 - r._1));
+  assert (pure (Seq.length s3 == hi - r._2));
+  
+  assert pure (squash (permutation s0 (Seq.append s1 (Seq.append s2 s3))));
+  
+  transfer_smaller_slice s lo lo r._1 r._3;
+  assert (pure (between_bounds s1 lb r._3));
+
+  transfer_equal_slice s lo r._1 r._2 r._3;
+  assert (pure (between_bounds s2 r._3 r._3));
+
+  transfer_larger_slice s lo r._2 hi r._3;
+  assert (pure (between_bounds s3 r._3 rb));
+  
   r
 }
 ```
@@ -338,88 +393,105 @@ fn partition_wrapper (a: A.array int) (lo: nat) (hi:(hi:nat{lo < hi - 1})) (n: n
 (** QuickSort **)
 
 unfold
-let pure_pre_quicksort (a: A.array int) (lo: nat) (hi:(hi:int{-1 <= hi - 1 /\ lo <= hi})) (lb rb: int) (n: nat) (s0: Seq.seq int)
-  = hi - 1 < n /\ between_bounds s0 lb rb /\ Seq.length s0 = hi - lo /\ SZ.fits n /\ A.length a = n /\ lo <= n /\ lb <= rb
+let pure_pre_quicksort (a: A.array int) (lo: nat) (hi:(hi:int{-1 <= hi - 1 /\ lo <= hi})) (lb rb: int) (s0: Seq.seq int)
+  = hi <= A.length a /\
+    between_bounds s0 lb rb /\
+    Seq.length s0 = hi - lo /\
+    SZ.fits (A.length a) /\
+    lo <= A.length a /\
+    lb <= rb
 
 unfold
-let pure_post_quicksort (a: A.array int) (lo: nat) (hi:(hi:int{-1 <= hi - 1 /\ lo <= hi})) (lb rb: int) (n: nat) (s0 s: Seq.seq int)
-  = hi - 1 < n /\ Seq.length s0 = hi - lo /\ Seq.length s = hi - lo /\ SZ.fits n /\ A.length a = n
-      /\ sorted s /\ between_bounds s lb rb /\ permutation s0 s
+let pure_post_quicksort (a: A.array int) (lo: nat) (hi:(hi:int{-1 <= hi - 1 /\ lo <= hi})) (lb rb: int) (s0 s: Seq.seq int)
+  = hi <= A.length a /\
+    Seq.length s0 = hi - lo /\
+    Seq.length s = hi - lo /\
+    SZ.fits (A.length a) /\
+    sorted s /\
+    between_bounds s lb rb /\
+    permutation s0 s
 
-(* Assuming recursion *)
 ```pulse
-fn quicksort' (a: A.array int) (lo: nat)
-(hi:(hi:int{-1 <= hi - 1 /\ lo <= hi}))
-(lb rb: int) (n: nat) (#s0: Ghost.erased (Seq.seq int))
-  requires A.pts_to_range a lo hi s0 ** pure (pure_pre_quicksort a lo hi lb rb n s0)
-  ensures exists* s. (A.pts_to_range a lo hi s ** pure (pure_post_quicksort a lo hi lb rb n s0 s))
-{ admit() }
+// this could probably be refactored into just joining two adjacent sorted arrays, and then define this calling that function twice
+ghost
+fn quicksort_proof
+  (a: A.array int)
+  (lo: nat)
+  (c1:(c1:nat{lo <= c1}))
+  (c2:(c2:nat{c1 <= c2}))
+  (hi:(hi:nat{c2 <= hi}))
+  (lb rb pivot : int)
+  (#s0: erased (Seq.seq int))
+  (s1 s2 s3 : Seq.seq int)
+  requires
+    (exists* s1'. (A.pts_to_range a lo c1 s1' ** pure (pure_post_quicksort a lo c1 lb pivot s1 s1'))) **
+    (exists* s3'. (A.pts_to_range a c2 hi s3' ** pure (pure_post_quicksort a c2 hi pivot rb s3 s3'))) **
+    A.pts_to_range a c1 c2 s2 **
+    pure (Seq.length s0 == hi - lo
+          /\ lb <= pivot /\ pivot <= rb
+          /\ permutation s0 (Seq.append s1 (Seq.append s2 s3))
+          /\ between_bounds s2 pivot pivot)
+  ensures
+    exists* s.
+      A.pts_to_range a lo hi s **
+      pure (pure_post_quicksort a lo hi lb rb s0 s)
+{
+  with s1'. assert (A.pts_to_range a lo c1 s1');
+  with s3'. assert (A.pts_to_range a c2 hi s3');
+
+  pts_to_range_join a c1 c2 hi;
+  pts_to_range_join a lo c1 hi;
+
+  let _ = append_permutations_3_squash s1 s2 s3 s1' s3' ();
+  let _ = lemma_sorted_append_squash s2 s3' pivot pivot pivot rb ();
+  let _ = lemma_sorted_append_squash s1' (Seq.append s2 s3') lb pivot pivot rb ();
+  ()
+}
 ```
 
-#push-options "--z3rlimit 50"
 ```pulse
-fn quicksort (a: A.array int) (lo: nat) (hi:(hi:int{-1 <= hi - 1 /\ lo <= hi})) (lb rb: int) (n: nat) (#s0: Ghost.erased (Seq.seq int))
-  requires A.pts_to_range a lo hi s0 ** pure (pure_pre_quicksort a lo hi lb rb n s0)
-  ensures exists* s. (A.pts_to_range a lo hi s ** pure (pure_post_quicksort a lo hi lb rb n s0 s))
-  // decreases hi + 1 - lo
+fn rec quicksort (a: A.array int) (lo: nat) (hi:(hi:int{-1 <= hi - 1 /\ lo <= hi})) (lb rb: int) (#s0: Ghost.erased (Seq.seq int))
+  requires A.pts_to_range a lo hi s0 ** pure (pure_pre_quicksort a lo hi lb rb s0)
+  ensures exists* s. (A.pts_to_range a lo hi s ** pure (pure_post_quicksort a lo hi lb rb s0 s))
 {
   if (lo < hi - 1)
   {
-    let r = partition_wrapper a lo hi n lb rb;
+    let r = partition_wrapper a lo hi lb rb;
     let pivot = r._3;
     with s1. assert (A.pts_to_range a lo r._1 s1);
     with s2. assert (A.pts_to_range a r._1 r._2 s2);
     with s3. assert (A.pts_to_range a r._2 hi s3);
-    //assert_prop (squash (permutation s0 (Seq.append s1 (Seq.append s2 s3))));
 
-    if (lo < hi + 1000) // worth parallelizing
+    if (lo + 1000 < hi) // worth parallelizing
+      ensures 
+          (exists* s. (A.pts_to_range a lo r._1 s ** pure (pure_post_quicksort a lo r._1 lb pivot s1 s))) **
+          (exists* s. (A.pts_to_range a r._2 hi s ** pure (pure_post_quicksort a r._2 hi pivot rb s3 s))) **
+          A.pts_to_range a r._1 r._2 s2 **
+          pure (Seq.length s0 == hi - lo
+                /\ lb <= pivot /\ pivot <= rb
+                /\ permutation s0 (Seq.append s1 (Seq.append s2 s3))
+                /\ between_bounds s2 pivot pivot)
     {
       parallel
-      requires (A.pts_to_range a lo r._1 s1 ** pure (pure_pre_quicksort a lo r._1 lb pivot n s1))
-          and (A.pts_to_range a r._2 hi s3 ** pure (pure_pre_quicksort a r._2 hi pivot rb n s3))
-      ensures (exists* s. (A.pts_to_range a lo r._1 s ** pure (pure_post_quicksort a lo r._1 lb pivot n s1 s)))
-          and (exists* s. (A.pts_to_range a r._2 hi s ** pure (pure_post_quicksort a r._2 hi pivot rb n s3 s)))
-      {
-        // termination check
-        assert_prop (hi - lo > (r._1 - 1) + 1 - lo);
-        quicksort' a lo r._1 lb pivot n;// (Ghost.hide s1);
-      }
-      {
-        // termination check
-        assert_prop (hi - lo > hi - r._2);
-        quicksort' a r._2 hi pivot rb n;
-      };
-
-      with s1'. assert (A.pts_to_range a lo r._1 s1');
-      with s3'. assert (A.pts_to_range a r._2 hi s3');
-      pts_to_range_join a lo r._1 r._2;
-      pts_to_range_join a lo r._2 hi;
-      Seq.append_assoc s1' s2 s3';
-      append_permutations_3 s1 s2 s3 s1' s3';
+        requires (A.pts_to_range a lo r._1 s1 ** pure (pure_pre_quicksort a lo r._1 lb pivot s1))
+            and (A.pts_to_range a r._2 hi s3 ** pure (pure_pre_quicksort a r._2 hi pivot rb s3))
+        ensures (exists* s. (A.pts_to_range a lo r._1 s ** pure (pure_post_quicksort a lo r._1 lb pivot s1 s)))
+            and (exists* s. (A.pts_to_range a r._2 hi s ** pure (pure_post_quicksort a r._2 hi pivot rb s3 s)))
+        { quicksort a lo r._1 lb pivot; }
+        { quicksort a r._2 hi pivot rb; };
       ()
-    }
-    else // sequential
-    {
-      // termination check
-      assert_prop (hi - lo > (r._1 - 1) + 1 - lo);
-      quicksort' a lo r._1 lb pivot n;
+    } else {
+      // else run sequentially
+      quicksort a lo r._1 lb pivot;
+      quicksort a r._2 hi pivot rb;
+    };
+    
+    with s1'. assert (A.pts_to_range a lo r._1 s1');
+    with s3'. assert (A.pts_to_range a r._2 hi s3');
+    
+    let _ = append_permutations_3_squash s1 s2 s3 s1' s3' ();
 
-      // termination check
-      assert_prop (hi - lo > hi - r._2);
-      quicksort' a r._2 hi pivot rb n;
-  
-      with s1'. assert (A.pts_to_range a lo r._1 s1');
-      with s3'. assert (A.pts_to_range a r._2 hi s3');
-      pts_to_range_join a lo r._1 r._2;
-      pts_to_range_join a lo r._2 hi;
-      Seq.append_assoc s1' s2 s3';
-      append_permutations_3 s1 s2 s3 s1' s3';
-      ()
-    }
-  }
-  else {
-    ()
+    quicksort_proof a lo r._1 r._2 hi lb rb pivot #s0 s1' s2 s3';
   }
 }
 ```
-#pop-options
