pulse/share/steel/examples/pulse/Quicksort.TaskParallel.fst
@@ -1,0 +1,133 @@
+(*
+   Copyright 2023 Microsoft Research
+
+   Licensed under the Apache License, Version 2.0 (the "License");
+   you may not use this file except in compliance with the License.
+   You may obtain a copy of the License at
+
+       http://www.apache.org/licenses/LICENSE-2.0
+
+   Unless required by applicable law or agreed to in writing, software
+   distributed under the License is distributed on an "AS IS" BASIS,
+   WITHOUT WARRANTIES OR CONDITIONS OF ANY KIND, either express or implied.
+   See the License for the specific language governing permissions and
+   limitations under the License.
+*)
+
+module QuickSort.TaskParallel
+open Pulse.Lib.Pervasives
+module A = Pulse.Lib.Array
+module R = Pulse.Lib.Reference
+module SZ = FStar.SizeT
+open Pulse.Lib.InvList
+
+module T = TaskPool
+open QuickSortParallel
+open Pulse.Lib.Par.Pledge
+
+let quicksort_post a lo hi s0 lb rb : vprop =
+  exists* s. (A.pts_to_range a lo hi s ** pure (pure_post_quicksort a lo hi lb rb s0 s))
+
+```pulse
+ghost
+fn join_alive_pledge (p:T.pool) (f:perm)
+  requires pledge is (T.pool_done p) (T.pool_alive #(half_perm f) p)
+        ** pledge is (T.pool_done p) (T.pool_alive #(half_perm f) p)
+  ensures pledge is (T.pool_done p) (T.pool_alive #f p)
+{
+  join_pledge #is #(T.pool_done p) (T.pool_alive #(half_perm f) p) (T.pool_alive #(half_perm f) p);
+
+  ghost fn
+    rewrite_pf
+      (_:unit)
+      requires
+        invlist_v is **
+        (T.pool_alive #(half_perm f) p ** T.pool_alive #(half_perm f) p)
+      ensures
+        invlist_v is **
+        (T.pool_alive #f p)
+    {
+      T.gather_alive p f;
+    };
+  
+  rewrite_pledge #is #(T.pool_done p)
+    (T.pool_alive #(half_perm f) p ** T.pool_alive #(half_perm f) p)
+    (T.pool_alive #f p)
+    rewrite_pf;
+}
+```
+
+(* NOTE: This is still a sketch as it is not spawning any of the sub tasks, but instead
+just calling sequentially. Already, however, pledge arithmetic is quite a big part
+of this proof. Spawning a subtask will require the use of split for permission
+accounting and complicate things further due to the extra invariant, unless we use
+the simple interface instead. *)
+```pulse
+fn rec t_quicksort
+  (p : T.pool)
+  (f : perm)
+  (a: A.array int)
+  (lo: nat) (hi:(hi:int{-1 <= hi - 1 /\ lo <= hi}))
+  (lb rb: int)
+  (#s0: Ghost.erased (Seq.seq int))
+  requires
+    T.pool_alive #f p **
+    A.pts_to_range a lo hi s0 **
+    pure (pure_pre_quicksort a lo hi lb rb s0)
+  ensures 
+    pledge [] (T.pool_done p) (T.pool_alive #f p) **
+    pledge [] (T.pool_done p) (quicksort_post a lo hi s0 lb rb)
+{
+  if (lo < hi - 1)
+  {
+    let r = partition_wrapper a lo hi lb rb;
+    let pivot = r._3;
+    with s1. assert (A.pts_to_range a lo r._1 s1);
+    with s2. assert (A.pts_to_range a r._1 r._2 s2);
+    with s3. assert (A.pts_to_range a r._2 hi s3);
+
+    T.share_alive p f;
+
+    t_quicksort p (half_perm f) a lo r._1 lb pivot;
+    t_quicksort p (half_perm f) a r._2 hi pivot rb;
+    
+    (* pledge arith *)
+    return_pledge [] (T.pool_done p) (A.pts_to_range a r._1 r._2 s2);
+    join_pledge #[] #(T.pool_done p)
+      (A.pts_to_range a r._1 r._2 s2)
+      (quicksort_post a lo r._1 s1 lb pivot);
+    join_pledge #[] #(T.pool_done p)
+      (A.pts_to_range a r._1 r._2 s2 ** quicksort_post a lo r._1 s1 lb pivot)
+      (quicksort_post a r._2 hi s3 pivot rb);
+      
+    ghost fn
+    rewrite_pf
+      (_:unit)
+      requires
+        emp ** // invs
+        (A.pts_to_range a r._1 r._2 s2 ** quicksort_post a lo r._1 s1 lb pivot ** quicksort_post a r._2 hi s3 pivot rb)
+      ensures
+        emp ** // invs
+        quicksort_post a lo hi s0 lb rb
+    {
+      unfold quicksort_post;
+      unfold quicksort_post;
+      quicksort_proof a lo r._1 r._2 hi lb rb pivot #s0 s1 s2 s3;
+      fold (quicksort_post a lo hi s0 lb rb);
+    };
+    rewrite_pledge #[] #(T.pool_done p)
+        (A.pts_to_range a r._1 r._2 s2 ** quicksort_post a lo r._1 s1 lb pivot ** quicksort_post a r._2 hi s3 pivot rb)
+        (quicksort_post a lo hi s0 lb rb)
+        rewrite_pf;
+
+    join_alive_pledge p f;
+
+    ()
+  } else {
+    return_pledge [] (T.pool_done p)
+      (exists* s. A.pts_to_range a lo hi s ** pure (pure_post_quicksort a lo hi lb rb s0 s));
+    return_pledge [] (T.pool_done p)
+      (T.pool_alive #f p);
+  }
+}
+```
